Define evaluation & using lemmas to prove rules

BBI.thy
@@ -2,21 +2,26 @@
     Author:     Tony Siu
 *)
 
-
 theory BBI
   imports Main
 begin
 
-section "BBI formula"
+section "BBI formula definiton"
 
+text \<open>First we define a variable which is indexed by natural number. 
+In this way we can genereate inifinte atomic proposition varaiables\<close>
 
-(* We define a variable which is indexed by natural number. In this way we can genereate inifinte atomic proposition varaiables *)
 datatype atom = P nat
 
-(* We now define a axiom which can evaluate atom to boolean *)
+text \<open>We now define a axiom which can evaluate atom to boolean without define how the function works
+We are generalising the method. This method allows Isabelle to cast an atomic variable to a boolean type\<close>
+
 axiomatization evalP :: "atom \<Rightarrow> bool" 
 
-(* With inifinte proposition variablse we can now define BBI formula. N.B. Capial M means the connective is a multiplicative connective *)
+text \<open>With inifinte proposition variables we can now define a BBI formula datatype.
+It is a recursive definition which includes symbols (both prefix and infix).
+The natural number next to the symbol indicate its precedence Isabell recommended range is >= 100\<close>
+
 datatype BBI_form = 
   Truth                     ("\<top>\<^sub>B")
   | Falsity                 ("\<bottom>\<^sub>B")
@@ -27,22 +32,30 @@ datatype BBI_form =
   | MCon BBI_form BBI_form  (infix "*\<^sub>B" 101)
   | Dis BBI_form BBI_form   (infix "\<or>\<^sub>B" 101)
   | Mdis BBI_form BBI_form  (infix "\<or>*\<^sub>B" 101)
+  | Imp  BBI_form BBI_form  (infix "\<rightarrow>\<^sub>B" 101)
+  | Mimp  BBI_form BBI_form  (infix "\<rightarrow>*\<^sub>B" 101)
 
-(* We now define a recursive evaluation to evaluate BBI formula to a boolean type*)
+text \<open>BBI_form is a custom mathematical object. Therefore it is difficult for Isabelle to prove any
+thing on this object. Therefore, we define a primitive recursive function to evaluate the formula to 
+boolean type\<close>
+
 primrec evalF :: "BBI_form \<Rightarrow> bool" where
   "evalF Truth = True"|
   "evalF Falsity = False"|
   "evalF (Atom p) = evalP p"|
   "evalF (\<not>\<^sub>B \<phi>) = (\<not>(evalF \<phi>))"|
   "evalF (~\<^sub>B \<phi>) =  (\<not>(evalF \<phi>))" |
-  "evalF (\<phi> \<and>\<^sub>B \<psi>) = ((evalF \<phi> )\<and>(evalF \<psi>))"|
-  "evalF (\<phi> *\<^sub>B \<psi>) = ((evalF \<phi> )\<and>(evalF \<psi>))"|
-  "evalF (\<phi> \<or>\<^sub>B \<psi>) = ((evalF \<phi> )\<or>(evalF \<psi>))"|
-  "evalF (\<phi> \<or>*\<^sub>B \<psi>) = ((evalF \<phi> )\<or>(evalF \<psi>))"
+  "evalF (\<phi> \<and>\<^sub>B \<psi>) = ((evalF \<phi>)\<and>(evalF \<psi>))"|
+  "evalF (\<phi> *\<^sub>B \<psi>) = ((evalF \<phi>)\<and>(evalF \<psi>))"|
+  "evalF (\<phi> \<or>\<^sub>B \<psi>) = ((evalF \<phi>)\<or>(evalF \<psi>))"|
+  "evalF (\<phi> \<or>*\<^sub>B \<psi>) = ((evalF \<phi>)\<or>(evalF \<psi>))"|
+  "evalF (\<phi> \<rightarrow>\<^sub>B \<psi>) = ((evalF \<phi>)\<longrightarrow>(evalF \<psi>))"|
+  "evalF (\<phi> \<rightarrow>*\<^sub>B \<psi>) = ((evalF \<phi>)\<longrightarrow>(evalF \<psi>))"
 
-definition "evaluation \<phi> \<equiv>  {\<xi>. \<xi>(evalF \<phi>)}"
 
-(* Here we have to create a lemma to show that negation of atomic BBI formula is equal to the negation of atomic proposition*)
+text \<open>The following evaluation is used to prove negation of atomic BBI formula can produce correct results
+As all BBI formula are borken down to a list of atomic propositions. Therefore, through a induction proof \<close>
+
 lemma negateAtom : 
   "evalF (Neg (Atom a)) \<Longrightarrow>  \<not>(evalP a)" 
   "evalF (Mneg (Atom a)) \<Longrightarrow>  \<not>(evalP a)"
@@ -52,16 +65,76 @@ lemma negateAtom :
   "evalF (Mneg Falsity) \<Longrightarrow> True" 
   by auto
 
-(* Basic Axiom for both CL and LM using auto proof through induction*)
+(* Missing BBI_form induction proof*)
+
+section "Axioms and Rules"
+text \<open>Now we try to implement CL and LM Rules through lemmas. 
+Due to our definition we can cast our BBI_form to a HOL object.
+All the rules can be proved using basic HOL rules without setting up customise proof notepad
+The auto prover help us to prove all LM rules.However, it does not show sub goals of proofs which is 
+opposite to CL lemmas\<close>
+
+text \<open>The following axiom rules apply to both CL and LM\<close>
 lemma Ax : "evalF f \<Longrightarrow> evalF f"
-  by auto
+  by blast
 
-section "Classical Logic Axioms and Rules"
+lemma MP : "\<lbrakk>evalF F \<Longrightarrow> evalF G; evalF G \<Longrightarrow> evalF H\<rbrakk> \<Longrightarrow> (evalF F \<Longrightarrow> evalF H)"
+  by blast
 
+subsection "Classical Logic Axioms and Rules"
+
+
+(* IL Rules*)
 lemma top: "evalF f \<Longrightarrow> True"
   by auto
 
 lemma bot: "False \<Longrightarrow> evalF f"
   by auto
 
+lemma disI :"\<lbrakk>evalF F; evalF G\<rbrakk> \<Longrightarrow> (evalF F \<or> evalF G)"
+  by blast
 
+lemma conI : "\<lbrakk>evalF F \<Longrightarrow> evalF G; evalF F \<Longrightarrow> evalF H\<rbrakk> \<Longrightarrow> evalF F \<Longrightarrow> evalF G \<and> evalF H" 
+  by blast
+
+lemma imp : "\<lbrakk>evalF F \<and> evalF G \<Longrightarrow> evalF H\<rbrakk> \<Longrightarrow> evalF F \<Longrightarrow> evalF G \<longrightarrow> evalF H"
+  by blast
+
+lemma conE1 : "\<lbrakk>evalF F \<and> evalF G\<rbrakk> \<Longrightarrow> evalF F"
+  by blast
+
+lemma conE2 : "\<lbrakk>evalF F \<and> evalF G\<rbrakk> \<Longrightarrow> evalF G"
+  by blast
+
+lemma disE : "\<lbrakk>evalF F \<Longrightarrow> evalF H; evalF G \<Longrightarrow> evalF H\<rbrakk> \<Longrightarrow> (evalF F \<or> evalF G \<Longrightarrow> evalF H)"
+  by blast
+
+
+(* CL rules*)
+lemma not : "\<lbrakk>\<not>(evalF F) \<Longrightarrow> evalF F ; evalF F \<Longrightarrow> \<not>(evalF F)\<rbrakk> \<Longrightarrow> False"
+  by blast
+
+lemma notnot : "\<lbrakk>\<not>\<not>(evalF F)\<rbrakk> \<Longrightarrow> evalF F"
+  by blast
+  
+subsection "Lambek Logic Axioms and Rules"
+
+(* Associative rule*)
+lemma assoc : "evalF (F  *\<^sub>B (G *\<^sub>B H)) \<longleftrightarrow> evalF ((F *\<^sub>B G)*\<^sub>B H)"
+  by auto
+
+lemma Mtruth : "evalF (F *\<^sub>B \<top>\<^sub>B ) \<longleftrightarrow> evalF F"
+  by auto
+
+(* Commutative rule*)
+lemma comm : "evalF (F *\<^sub>B G) \<Longrightarrow> evalF(G *\<^sub>B F)"
+  by auto
+
+lemma MconI : "\<lbrakk>evalF F\<^sub>1 \<Longrightarrow> evalF G\<^sub>1 ;evalF F\<^sub>2 \<Longrightarrow> evalF G\<^sub>2\<rbrakk> \<Longrightarrow> (evalF (F\<^sub>1 *\<^sub>B F\<^sub>2) \<Longrightarrow> evalF (G\<^sub>1 *\<^sub>B G\<^sub>2))"
+  by auto
+
+lemma Mimp : "\<lbrakk>evalF (F *\<^sub>B G) \<Longrightarrow> evalF H\<rbrakk> \<Longrightarrow> (evalF F \<Longrightarrow> evalF(G \<rightarrow>*\<^sub>B H))"
+  by auto
+
+
+ 
